theories/Map.v
@@ -9,6 +9,7 @@ Module Env <: FMapInterface.S := FMapAVL.Make OrderedTypeEx.Nat_as_OT.
 Definition map := Env.t.
 
 Definition one {V} (x: nat) (v: V) := Env.add x v (Env.empty _).
+Definition add {V}: nat -> V -> Env.t V -> Env.t V := @Env.add _.
 Definition merge {V}: Env.t V -> Env.t V -> Env.t V := Env.map2 (fun x y => if x is Some _ then x else y).
 Definition minus {V}: nat -> Env.t V -> Env.t V := @Env.remove _.
 Definition find {V}: nat -> Env.t V -> option V := @Env.find _.
