theories/Spec.v
@@ -86,12 +86,6 @@ Definition appctx_context_ctx_context (context_ctx5:context_ctx) (context5:conte
   | (e_app_r E) => (E_app context5 E)
 end.
 
-Function I (e: list _) E :=
-  match e with
-  | cons h t => appctx_context_ctx_context h (I t E)
-  |  _ => E
-  end.
-
 
 (** subrules *)
 Fixpoint is_term_norm_of_term (v5:term) : bool :=
@@ -139,10 +133,9 @@ end.
 Inductive judge_E : environment -> context -> type -> Prop :=    (* defn judge_E *)
  | JE_var : forall (x:var) (t:type),
      judge_E  (Map.one  x   t )  (E_var x) t
- | JE_abs : forall (e_list:list context_ctx) (G:environment) (x:var) (t1 t2:type),
-     Map.find x G = Some t1  ->
-     judge_E G  (I  e_list   (E_var x) )  t2 ->
-     judge_E  (Map.minus  x   G )  (E_all x t1  (I  e_list   (E_var x) ) ) (t_prod t1 t2)
+ | JE_abs : forall (G:environment) (x:var) (t1:type) (E:context) (t2:type),
+     judge_E  (Map.add  x   t1   G )  E t2 ->
+     judge_E G (E_all x t1 E) (t_prod t1 t2)
  | JE_app : forall (G1 G2:environment) (E1 E2:context) (t2 t1:type),
      judge_E G1 E1 (t_prod t1 t2) ->
      judge_E G2 E2 t1 ->
@@ -171,8 +164,8 @@ with sat : context -> term -> Prop :=    (* defn sat *)
 
 (* defns eval *)
 Inductive step_E : context -> context -> Prop :=    (* defn step_E *)
- | stepE_beta : forall (e_list:list context_ctx) (x:var) (t:type) (E:context),
-     step_E (E_app  ( (E_all x t  (I  e_list   (E_var x) ) ) )  E)  (I  e_list   E ) 
+ | stepE_beta : forall (x:var) (t:type) (E E':context),
+     step_E (E_app  ( (E_all x t E) )  E')  (subst_context  E'   x   E ) 
  | stepE_ctx : forall (e:context_ctx) (E E':context),
      step_E E E' ->
      step_E  (appctx_context_ctx_context  e   E )   (appctx_context_ctx_context  e   E' ) 
